update morphisms and systems to enable contract sums with the null contract

execution/theories/ContractMorphisms.v
@@ -17,6 +17,8 @@ From ConCert.Utils Require Import RecordUpdate.
 
 (* Axiom todo : string -> forall {A}, A. *)
 
+(* TODO USE `GENERALIZE VARIABLE` SYNTAX TO GET RID OF ALL THE IMPLICIT NOTATION *)
+
 (* some auxiliary functions *)
 Definition curry_3 {A B C D : Type} (f : A * B * C -> D) : A -> B -> C -> D := 
     (compose curry curry) f.
@@ -30,15 +32,14 @@ Definition uncurry_4 {A B C D E : Type} (f : A -> B -> C -> D -> E) : A * B * C 
 Section ContractMorphisms.
 Context { Base : ChainBase }.
 
+
 (** First, a definition of a Contract Morphism, which is a function between contracts *)
 Section MorphismDefinition.
+Context `{Serializable Msg}  `{Serializable Setup}  `{Serializable State}  `{Serializable Error}
+    `{Serializable Msg'} `{Serializable Setup'} `{Serializable State'} `{Serializable Error'}.
 
 (** The init component *)
-Record InitCM
-    { Setup Setup' Msg Msg' State State' Error Error' : Type }
-    `{Serializable Msg}  `{Serializable Setup}  `{Serializable State}  `{Serializable Error}
-    `{Serializable Msg'} `{Serializable Setup'} `{Serializable State'} `{Serializable Error'}
-    (C : Contract Setup Msg State Error) (C' : Contract Setup' Msg' State' Error') 
+Record InitCM (C : Contract Setup Msg State Error) (C' : Contract Setup' Msg' State' Error') 
     := build_init_cm {
         (* transform inputs/outputs of the init function *)
         init_inputs : Chain * ContractCallContext * Setup -> 
@@ -52,11 +53,7 @@ Record InitCM
     }.
 
 (** The receive component *)
-Record RecvCM
-    { Setup Setup' Msg Msg' State State' Error Error' : Type }
-    `{Serializable Msg}  `{Serializable Setup}  `{Serializable State}  `{Serializable Error}
-    `{Serializable Msg'} `{Serializable Setup'} `{Serializable State'} `{Serializable Error'}
-    (C : Contract Setup Msg State Error) (C' : Contract Setup' Msg' State' Error') := 
+Record RecvCM (C : Contract Setup Msg State Error) (C' : Contract Setup' Msg' State' Error') := 
     build_recv_cm {
         (* transform inputs/outputs of the receive function *)
         recv_inputs : Chain * ContractCallContext * State * option Msg -> 
@@ -72,9 +69,6 @@ Record RecvCM
 
 (** The definition *)
 Record ContractMorphism 
-    { Setup Setup' Msg Msg' State State' Error Error' : Type }
-    `{Serializable Msg}  `{Serializable Setup}  `{Serializable State}  `{Serializable Error}
-    `{Serializable Msg'} `{Serializable Setup'} `{Serializable State'} `{Serializable Error'}
     (C  : Contract Setup  Msg  State  Error) 
     (C' : Contract Setup' Msg' State' Error') := 
     build_cm {
@@ -86,26 +80,18 @@ End MorphismDefinition.
 
 
 Section MorphismUtilities.
-
-Definition init_cm 
-    { Setup Setup' Msg Msg' State State' Error Error' : Type }
-    `{Serializable Msg}  `{Serializable Setup}  `{Serializable State}  `{Serializable Error}
+Context `{Serializable Msg}  `{Serializable Setup}  `{Serializable State}  `{Serializable Error}
     `{Serializable Msg'} `{Serializable Setup'} `{Serializable State'} `{Serializable Error'}
-    {C : Contract Setup Msg State Error} {C' : Contract Setup' Msg' State' Error'} 
-    (f : ContractMorphism C C') : InitCM C C' := 
+    {C : Contract Setup Msg State Error} {C' : Contract Setup' Msg' State' Error'}.
+
+Definition init_cm (f : ContractMorphism C C') : InitCM C C' := 
     cm_init C C' f.
-Definition recv_cm 
-        { Setup Setup' Msg Msg' State State' Error Error' : Type }
-        `{Serializable Msg}  `{Serializable Setup}  `{Serializable State}  `{Serializable Error}
-        `{Serializable Msg'} `{Serializable Setup'} `{Serializable State'} `{Serializable Error'}
-        {C : Contract Setup Msg State Error} {C' : Contract Setup' Msg' State' Error'} 
-    (f : ContractMorphism C C') : RecvCM C C' := 
+Definition recv_cm (f : ContractMorphism C C') : RecvCM C C' := 
     cm_recv C C' f.
 Definition id_fun (A : Type) : A -> A := @id A.
 
 (* the coherence conditions for constructing non-opaque morphisms *)
 Definition init_morphs_commute  
-    { Setup Setup' State State' Error Error' : Type}
     (init  : Chain -> ContractCallContext -> Setup  -> result State  Error)
     (init' : Chain -> ContractCallContext -> Setup' -> result State' Error')
     (init_inputs : Chain * ContractCallContext * Setup -> 
@@ -116,7 +102,6 @@ Definition init_morphs_commute
         init_outputs (uncurry_3 init x).
 
 Definition recv_morphs_commute 
-    { Msg Msg' State State' Error Error' : Type }
     (recv  : Chain -> ContractCallContext -> State  -> option Msg  -> 
         result (State  * list ActionBody) Error)
     (recv' : Chain -> ContractCallContext -> State' -> option Msg' -> 
@@ -134,17 +119,16 @@ End MorphismUtilities.
 
 (** The Identity Contract Morphism *)
 Section IdentityMorphism.
+Context { Setup Msg State Error : Type }
+  `{Serializable Msg}  `{Serializable Setup}  `{Serializable State} `{Serializable Error}.
 
 (* an opaque construction *)
-Definition id_cm_opaque 
-    { Setup Msg State Error : Type }
-    `{Serializable Msg}  `{Serializable Setup}  `{Serializable State} `{Serializable Error}
-    (C : Contract Setup Msg State Error) : ContractMorphism C C.
+Definition id_cm_opaque (C : Contract Setup Msg State Error) : ContractMorphism C C.
 Proof.
     constructor.
     -   set (init_inputs  := id_fun (Chain * ContractCallContext * Setup)).
         set (init_outputs := id_fun (result State Error)).
-        apply (build_init_cm Setup Setup Msg Msg State State Error Error H H0 H1 H2 H H0 H1 H2 C C init_inputs init_outputs).
+        apply (build_init_cm C C init_inputs init_outputs).
         intro. destruct x. destruct p.
         unfold uncurry_3. 
         unfold init_inputs. unfold init_outputs. 
@@ -152,7 +136,7 @@ Proof.
         reflexivity.
     -   set (recv_inputs  := id_fun (Chain * ContractCallContext * State * option Msg)).
         set (recv_outputs := id_fun (result (State * list ActionBody) Error)).
-        apply (build_recv_cm Setup Setup Msg Msg State State Error Error H H0 H1 H2 H H0 H1 H2 C C recv_inputs recv_outputs).
+        apply (build_recv_cm C C recv_inputs recv_outputs).
         intro. destruct x. repeat destruct p.
         unfold uncurry_4. 
         unfold recv_inputs. unfold recv_outputs. 
@@ -161,20 +145,14 @@ Proof.
 Qed.
 
 (* an explicit construction *)
-Lemma init_commutes_id 
-    { Setup Msg State Error : Type }
-    `{Serializable Msg}  `{Serializable Setup}  `{Serializable State} `{Serializable Error}
-    (C : Contract Setup Msg State Error) :
+Lemma init_commutes_id (C : Contract Setup Msg State Error) :
     init_morphs_commute 
         C.(init) C.(init) 
         (id_fun (Chain * ContractCallContext * Setup)) 
         (id_fun (result State Error)).
-Proof. intro. auto. Qed.
+Proof. now intro. Qed.
 
-Definition id_cm_init 
-    { Setup Msg State Error : Type }
-    `{Serializable Msg}  `{Serializable Setup}  `{Serializable State} `{Serializable Error}
-    (C : Contract Setup Msg State Error) :
+Definition id_cm_init (C : Contract Setup Msg State Error) :
     InitCM C C := {|
         init_inputs  := id_fun (Chain * ContractCallContext * Setup) ;
         init_outputs := id_fun (result State Error) ;
@@ -182,20 +160,14 @@ Definition id_cm_init
         init_commutes := init_commutes_id C ;
     |}.
 
-Lemma recv_commutes_id 
-    { Setup Msg State Error : Type }
-    `{Serializable Msg}  `{Serializable Setup}  `{Serializable State} `{Serializable Error}
-    (C : Contract Setup Msg State Error) :
+Lemma recv_commutes_id (C : Contract Setup Msg State Error) :
     recv_morphs_commute 
         C.(receive) C.(receive) 
         (id_fun (Chain * ContractCallContext * State * option Msg)) 
         (id_fun (result (State * list ActionBody) Error)).
-Proof. intro. auto. Qed.
+Proof. now intro. Qed.
 
-Definition id_cm_recv 
-    { Setup Msg State Error : Type }
-    `{Serializable Msg}  `{Serializable Setup}  `{Serializable State} `{Serializable Error}
-    (C : Contract Setup Msg State Error) : RecvCM C C := {|
+Definition id_cm_recv (C : Contract Setup Msg State Error) : RecvCM C C := {|
         recv_inputs := id_fun (Chain * ContractCallContext * State * option Msg) ;
         recv_outputs := id_fun (result (State * list ActionBody) Error) ;
         (* proof of commutativity *)
@@ -203,10 +175,7 @@ Definition id_cm_recv
     |}.
 
 (* * the identity morphism *)
-Definition id_cm 
-    { Setup Msg State Error : Type }
-    `{Serializable Msg}  `{Serializable Setup}  `{Serializable State} `{Serializable Error}
-    (C : Contract Setup Msg State Error) : ContractMorphism C C := {|
+Definition id_cm (C : Contract Setup Msg State Error) : ContractMorphism C C := {|
         cm_init := id_cm_init C ;
         cm_recv := id_cm_recv C ;
     |}.
@@ -215,12 +184,12 @@ End IdentityMorphism.
 
 (** Deriving equality of Contract Morphisms *)
 Section EqualityOfMorphisms.
+Context     { Setup Setup' Msg Msg' State State' Error Error' : Type }
+`{Serializable Msg}  `{Serializable Setup}  `{Serializable State}  `{Serializable Error}
+`{Serializable Msg'} `{Serializable Setup'} `{Serializable State'} `{Serializable Error'}
+{C : Contract Setup Msg State Error} {C' : Contract Setup' Msg' State' Error'}.
 
-Lemma is_eq_cm 
-    { Setup Setup' Msg Msg' State State' Error Error' : Type }
-    `{Serializable Msg}  `{Serializable Setup}  `{Serializable State}  `{Serializable Error}
-    `{Serializable Msg'} `{Serializable Setup'} `{Serializable State'} `{Serializable Error'}
-    {C : Contract Setup Msg State Error} {C' : Contract Setup' Msg' State' Error'} :
+Lemma is_eq_cm :
     forall (f g : ContractMorphism C C'), 
     init_cm f = init_cm g -> 
     recv_cm f = recv_cm g -> 
@@ -228,41 +197,43 @@ Lemma is_eq_cm
 Proof.
     intros f g init_eq recv_eq.
     destruct f. destruct g. f_equal.
-    - unfold init_cm in init_eq. unfold cm_init in init_eq.
-      exact init_eq.
-    - unfold recv_cm in recv_eq. unfold cm_recv in recv_eq.
-      exact recv_eq.
+    - unfold init_cm in init_eq. 
+      now unfold cm_init in init_eq.
+    - unfold recv_cm in recv_eq. 
+      now unfold cm_recv in recv_eq.
 Qed.
 
-Lemma is_eq_cm_init
-    { Setup Setup' Msg Msg' State State' Error Error' : Type }
-    `{Serializable Msg}  `{Serializable Setup}  `{Serializable State}  `{Serializable Error}
-    `{Serializable Msg'} `{Serializable Setup'} `{Serializable State'} `{Serializable Error'}
-    {C : Contract Setup Msg State Error} {C' : Contract Setup' Msg' State' Error'} :
+Lemma is_eq_cm_init :
     forall (f g : ContractMorphism C C'),
     (init_inputs C C' (init_cm f)) = (init_inputs C C' (init_cm g)) -> 
     (init_outputs C C' (init_cm f)) = (init_outputs C C' (init_cm g)) -> 
     init_cm f = init_cm g.
 Proof.
-    intros f g. destruct f. destruct g. simpl.
-    destruct cm_init0. destruct cm_init1. simpl. 
-    intros inputs_eq outputs_eq. subst. f_equal.
+    intros f g. 
+    destruct f, g. 
+    simpl.
+    destruct cm_init0, cm_init1. 
+    simpl. 
+    intros inputs_eq outputs_eq. 
+    subst. 
+    f_equal.
     apply proof_irrelevance.
 Qed.
 
-Lemma is_eq_cm_recv 
-    { Setup Setup' Msg Msg' State State' Error Error' : Type }
-    `{Serializable Msg}  `{Serializable Setup}  `{Serializable State}  `{Serializable Error}
-    `{Serializable Msg'} `{Serializable Setup'} `{Serializable State'} `{Serializable Error'}
-    {C : Contract Setup Msg State Error} {C' : Contract Setup' Msg' State' Error'} :
+Lemma is_eq_cm_recv :
     forall (f g : ContractMorphism C C'),
     (recv_inputs C C' (recv_cm f)) = (recv_inputs C C' (recv_cm g)) -> 
     (recv_outputs C C' (recv_cm f)) = (recv_outputs C C' (recv_cm g)) -> 
     recv_cm f = recv_cm g.
 Proof.
-    intros f g. destruct f. destruct g. simpl.
-    destruct cm_recv0. destruct cm_recv1. simpl.
-    intros inputs_eq outputs_eq. subst. f_equal.
+    intros f g. 
+    destruct f, g. 
+    simpl.
+    destruct cm_recv0, cm_recv1. 
+    simpl.
+    intros inputs_eq outputs_eq. 
+    subst. 
+    f_equal.
     apply proof_irrelevance.
 Qed.
 
@@ -271,18 +242,16 @@ End EqualityOfMorphisms.
 
 (** An explicit construction of the composition of two morphisms *)
 Section MorphismComposition.
+Context { Setup Setup' Setup'' Msg Msg' Msg'' State State' State'' Error Error' Error'' : Type }
+  `{Serializable Msg} `{Serializable Setup} `{Serializable State} `{Serializable Error}
+  `{Serializable Msg'} `{Serializable Setup'} `{Serializable State'} `{Serializable Error'}
+  `{Serializable Msg''} `{Serializable Setup''} `{Serializable State''} `{Serializable Error''}
+  { C : Contract Setup Msg State Error } 
+  { C' : Contract Setup' Msg' State' Error' }
+  { C'' : Contract Setup'' Msg'' State'' Error'' }.
 
 (** The Init component *)
-Lemma compose_commutes_init 
-    { Setup Setup' Setup'' Msg Msg' Msg'' State State' State'' Error Error' Error'' : Type }
-    `{Serializable Msg}    `{Serializable Setup}    `{Serializable State}    `{Serializable Error}
-    `{Serializable Msg'}   `{Serializable Setup'}   `{Serializable State'}   `{Serializable Error'}
-    `{Serializable Msg''}  `{Serializable Setup''}  `{Serializable State''}  `{Serializable Error''}
-    { C : Contract Setup Msg State Error } 
-    { C' : Contract Setup' Msg' State' Error' }
-    { C'' : Contract Setup'' Msg'' State'' Error'' } 
-    (g : ContractMorphism C' C'')
-    (f : ContractMorphism C  C') :
+Lemma compose_commutes_init (g : ContractMorphism C' C'') (f : ContractMorphism C  C') :
     init_morphs_commute 
         C.(init) 
         C''.(init)
@@ -296,16 +265,7 @@ Proof.
 Qed.
 
 (** The Recv component *)
-Lemma compose_commutes_recv
-    { Setup Setup' Setup'' Msg Msg' Msg'' State State' State'' Error Error' Error'' : Type }
-    `{Serializable Msg}    `{Serializable Setup}    `{Serializable State}    `{Serializable Error}
-    `{Serializable Msg'}   `{Serializable Setup'}   `{Serializable State'}   `{Serializable Error'}
-    `{Serializable Msg''}  `{Serializable Setup''}  `{Serializable State''}  `{Serializable Error''}
-    { C : Contract Setup Msg State Error } 
-    { C' : Contract Setup' Msg' State' Error' }
-    { C'' : Contract Setup'' Msg'' State'' Error'' } 
-    (g : ContractMorphism C' C'')
-    (f : ContractMorphism C  C') :
+Lemma compose_commutes_recv (g : ContractMorphism C' C'') (f : ContractMorphism C  C') :
     recv_morphs_commute 
         C.(receive)
         C''.(receive)
@@ -319,16 +279,8 @@ Proof.
 Qed.
 
 (** Composition *)
-Definition composition_cm 
-    { Setup Setup' Setup'' Msg Msg' Msg'' State State' State'' Error Error' Error'' : Type }
-    `{Serializable Msg}    `{Serializable Setup}    `{Serializable State}    `{Serializable Error}
-    `{Serializable Msg'}   `{Serializable Setup'}   `{Serializable State'}   `{Serializable Error'}
-    `{Serializable Msg''}  `{Serializable Setup''}  `{Serializable State''}  `{Serializable Error''}
-    { C : Contract Setup Msg State Error } 
-    { C' : Contract Setup' Msg' State' Error' }
-    { C'' : Contract Setup'' Msg'' State'' Error'' } 
-    (g : ContractMorphism C' C'')
-    (f : ContractMorphism C  C') : ContractMorphism C C'' := 
+Definition composition_cm (g : ContractMorphism C' C'') (f : ContractMorphism C  C') 
+    : ContractMorphism C C'' := 
     let compose_init := {|
         init_inputs  := compose (init_inputs  C' C'' (init_cm g)) (init_inputs  C C' (init_cm f)) ;
         init_outputs := compose (init_outputs C' C'' (init_cm g)) (init_outputs C C' (init_cm f)) ;
@@ -346,49 +298,48 @@ Definition composition_cm
         cm_recv := compose_recv ;
     |}.
 
+End MorphismComposition.
+
+Section CompositionEGs.
+Context { Setup Setup' Setup'' Setup''' Msg Msg' Msg'' Msg''' 
+State State' State'' State''' 
+Error Error' Error'' Error''' : Type }
+`{Serializable Msg} `{Serializable Setup} `{Serializable State} `{Serializable Error}
+`{Serializable Msg'} `{Serializable Setup'} `{Serializable State'} `{Serializable Error'}
+`{Serializable Msg''} `{Serializable Setup''} `{Serializable State''} `{Serializable Error''}
+`{Serializable Msg'''} `{Serializable Setup'''} `{Serializable State'''} `{Serializable Error'''}
+{ C : Contract Setup Msg State Error } 
+{ C' : Contract Setup' Msg' State' Error' }
+{ C'' : Contract Setup'' Msg'' State'' Error'' }
+{ C''' : Contract Setup''' Msg''' State''' Error''' }.
+
 (** Composition with the Identity morphism is trivial *)
-Proposition composition_id_cm_left 
-    { Setup Setup' Msg Msg' State State' Error Error' : Type }
-    `{Serializable Msg}  `{Serializable Setup}  `{Serializable State}  `{Serializable Error}
-    `{Serializable Msg'} `{Serializable Setup'} `{Serializable State'} `{Serializable Error'}
-    {C : Contract Setup Msg State Error} {C' : Contract Setup' Msg' State' Error'} :
+Proposition composition_id_cm_left :
     forall (f : ContractMorphism C C'), 
     (composition_cm (id_cm C') f) = f.
 Proof.
-    intros. unfold composition_cm. unfold id_cm. simpl.
+    intros. 
+    unfold composition_cm, id_cm. 
+    simpl.
     apply is_eq_cm; simpl.
     -   apply (is_eq_cm_init (composition_cm (id_cm C') f) f); auto.
     -   apply (is_eq_cm_recv (composition_cm (id_cm C') f) f); auto.
 Qed.
 
-Proposition composition_id_cm_right 
-    { Setup Setup' Msg Msg' State State' Error Error' : Type }
-    `{Serializable Msg}  `{Serializable Setup}  `{Serializable State}  `{Serializable Error}
-    `{Serializable Msg'} `{Serializable Setup'} `{Serializable State'} `{Serializable Error'}
-    {C : Contract Setup Msg State Error} {C' : Contract Setup' Msg' State' Error'} :
+Proposition composition_id_cm_right :
     forall (f : ContractMorphism C C'), 
     (composition_cm f (id_cm C)) = f.
 Proof.
-    intros. unfold composition_cm. unfold id_cm. simpl.
+    intros. 
+    unfold composition_cm, id_cm. 
+    simpl.
     apply is_eq_cm; simpl. 
     + apply (is_eq_cm_init (composition_cm f (id_cm C)) f); auto.
     + apply (is_eq_cm_recv (composition_cm f (id_cm C)) f); auto.
 Qed.
 
 (** Composition is associative *)
-Proposition composition_assoc_cm 
-    { Setup Setup' Setup'' Setup''' 
-    Msg   Msg'   Msg''   Msg''' 
-    State State' State'' State''' 
-    Error Error' Error'' Error''' : Type }
-    `{Serializable Msg} `{Serializable Setup} `{Serializable State} `{Serializable Error}
-    `{Serializable Msg'} `{Serializable Setup'} `{Serializable State'} `{Serializable Error'}
-    `{Serializable Msg''} `{Serializable Setup''} `{Serializable State''} `{Serializable Error''}
-    `{Serializable Msg'''} `{Serializable Setup'''} `{Serializable State'''} `{Serializable Error'''}
-    { C : Contract Setup Msg State Error } 
-    { C' : Contract Setup' Msg' State' Error' }
-    { C'' : Contract Setup'' Msg'' State'' Error'' }
-    { C''' : Contract Setup''' Msg''' State''' Error''' } :
+Proposition composition_assoc_cm :
     forall 
     (f : ContractMorphism C C') 
     (g : ContractMorphism C' C'') 
@@ -398,47 +349,41 @@ Proposition composition_assoc_cm
 Proof.
     intros.
     unfold composition_cm. simpl. apply is_eq_cm.
-    -   apply 
+    -   now apply 
         (is_eq_cm_init 
             (composition_cm h (composition_cm g f))
-            (composition_cm (composition_cm h g) f)); auto.
-    -   apply 
+            (composition_cm (composition_cm h g) f)).
+    -   now apply 
         (is_eq_cm_recv 
             (composition_cm h (composition_cm g f))
-            (composition_cm (composition_cm h g) f)); auto.
+            (composition_cm (composition_cm h g) f)).
 Qed.
 
-End MorphismComposition.
+End CompositionEGs.
 
 
 (** We will treat various type of contract morphisms, starting with isomorphisms. *)
-Section Isomorphisms.
+Section IsomorphismDefinition.
+Context { Setup Setup' Msg Msg' State State' Error Error' : Type }
+`{Serializable Msg}  `{Serializable Setup}  `{Serializable State}  `{Serializable Error}
+`{Serializable Msg'} `{Serializable Setup'} `{Serializable State'} `{Serializable Error'}
+{C : Contract Setup Msg State Error} {C' : Contract Setup' Msg' State' Error'}.
 
 Definition is_iso {A B : Type} (f : A -> B) (g : B -> A) : Prop := 
     compose g f = @id A /\ compose f g = @id B.
 
 Lemma is_iso_reflexive {A B : Type} (f : A -> B) (g : B -> A) : 
     is_iso f g -> is_iso g f.
-Proof. unfold is_iso. intro. destruct H. auto. Qed.
+Proof. unfold is_iso. intro H_is_iso. now destruct H_is_iso. Qed.
 
 Definition is_iso_cm 
-        { Setup Setup' Msg Msg' State State' Error Error' : Type }
-        `{Serializable Msg}  `{Serializable Setup}  `{Serializable State}  `{Serializable Error}
-        `{Serializable Msg'} `{Serializable Setup'} `{Serializable State'} `{Serializable Error'}
-        {C : Contract Setup Msg State Error} {C' : Contract Setup' Msg' State' Error'} 
     (f : ContractMorphism C C')
     (g : ContractMorphism C' C) : Prop := 
     composition_cm g f = id_cm C /\ 
     composition_cm f g = id_cm C'.
 
-Lemma iso_cm_components 
-        { Setup Setup' Msg Msg' State State' Error Error' : Type }
-        `{Serializable Msg}  `{Serializable Setup}  `{Serializable State}  `{Serializable Error}
-        `{Serializable Msg'} `{Serializable Setup'} `{Serializable State'} `{Serializable Error'}
-        {C : Contract Setup Msg State Error} {C' : Contract Setup' Msg' State' Error'} :
-    forall 
-        (f : ContractMorphism C C')
-        (g : ContractMorphism C' C),
+Lemma iso_cm_components :
+    forall (f : ContractMorphism C C') (g : ContractMorphism C' C),
     is_iso (init_inputs  C C' (init_cm f)) (init_inputs  C' C (init_cm g)) /\
     is_iso (init_outputs C C' (init_cm f)) (init_outputs C' C (init_cm g)) /\
     is_iso (recv_inputs  C C' (recv_cm f)) (recv_inputs  C' C (recv_cm g)) /\
@@ -479,26 +424,11 @@ Proof.
         auto.
 Qed.
 
-Lemma iso_cm_reflexive
-        { Setup Setup' Msg Msg' State State' Error Error' : Type }
-        `{Serializable Msg}  `{Serializable Setup}  `{Serializable State}  `{Serializable Error}
-        `{Serializable Msg'} `{Serializable Setup'} `{Serializable State'} `{Serializable Error'}
-        {C : Contract Setup Msg State Error} {C' : Contract Setup' Msg' State' Error'}
-    (f : ContractMorphism C C')
-    (g : ContractMorphism C' C) : 
-    is_iso_cm f g -> 
-    is_iso_cm g f.
-Proof.
-    intro. apply iso_cm_components in H7. 
-    apply iso_cm_components. destruct H7.
-    apply is_iso_reflexive in H7. split; try exact H7. destruct H8.
-    apply is_iso_reflexive in H8. split; try exact H8. destruct H9.
-    apply is_iso_reflexive in H9. split; try exact H9.
-    apply is_iso_reflexive in H10. exact H10.
-Qed.
+End IsomorphismDefinition.
 
-Lemma composition_iso_cm 
-        { Setup Setup' Setup'' Setup''' 
+
+Section Isomorphisms.
+Context { Setup Setup' Setup'' Setup''' 
         Msg   Msg'   Msg''   Msg''' 
         State State' State'' State''' 
         Error Error' Error'' Error''' : Type }
@@ -509,7 +439,31 @@ Lemma composition_iso_cm
         { C : Contract Setup Msg State Error } 
         { C' : Contract Setup' Msg' State' Error' }
         { C'' : Contract Setup'' Msg'' State'' Error'' }
-        { C''' : Contract Setup''' Msg''' State''' Error''' }
+        { C''' : Contract Setup''' Msg''' State''' Error''' }.
+
+Definition contracts_isomorphic 
+    (C : Contract Setup Msg State Error)
+    (C' : Contract Setup' Msg' State' Error') : Prop := 
+    exists (f : ContractMorphism C C') (g : ContractMorphism C' C),
+    is_iso_cm f g.
+
+Lemma iso_cm_reflexive (f : ContractMorphism C C') (g : ContractMorphism C' C) : 
+    is_iso_cm f g -> 
+    is_iso_cm g f.
+Proof.
+    intro H_is_iso.
+    apply iso_cm_components in H_is_iso.
+    apply iso_cm_components. 
+    destruct H_is_iso as [H_ind_iso H_is_iso].
+    do 2 (apply is_iso_reflexive in H_ind_iso;
+    split; 
+    try exact H_ind_iso; 
+    clear H_ind_iso;
+    destruct H_is_iso as [H_ind_iso H_is_iso]).
+    split; now apply is_iso_reflexive.
+Qed.
+
+Lemma composition_iso_cm 
     (f : ContractMorphism C C')
     (g : ContractMorphism C' C'')
     (f' : ContractMorphism C' C)
@@ -548,10 +502,8 @@ Definition is_inj_cm
     (f : ContractMorphism C C') : Prop := 
     (* init morphisms inject *)
     is_inj (init_inputs  C C' (init_cm f)) /\
-    is_inj (init_outputs C C' (init_cm f)) /\
     (* recv morphisms inject *)
-    is_inj (recv_inputs  C C' (recv_cm f)) /\
-    is_inj (recv_outputs C C' (recv_cm f)).
+    is_inj (recv_inputs  C C' (recv_cm f)).
 
 Definition contract_embeds 
         { Setup Setup' Msg Msg' State State' Error Error' : Type }
@@ -576,11 +528,9 @@ Definition is_surj_cm
         {C : Contract Setup Msg State Error} {C' : Contract Setup' Msg' State' Error'}
     (f : ContractMorphism C C') : Prop := 
     (* init morphisms surject *)
-    is_surj (init_inputs C C' (init_cm f)) /\ 
-    is_surj (init_outputs C C' (init_cm f)) /\
+    is_surj (init_inputs C C' (init_cm f)) /\
     (* recv morphisms surject *)
-    is_surj (recv_inputs C C' (recv_cm f)) /\
-    is_surj (recv_outputs C C' (recv_cm f)).
+    is_surj (recv_inputs C C' (recv_cm f)).
 
 Definition contract_surjects 
         { Setup Setup' Msg Msg' State State' Error Error' : Type }
@@ -595,8 +545,8 @@ End Surjections.
 (** We have some interesting categorical properties, including the existence of a terminal
     contract. (Note that we have not yet proved uniqueness of the terminal morphism.) *)
 Section TerminalContract.
-    Import ListNotations.
-    Set Nonrecursive Elimination Schemes.
+Import ListNotations.
+Set Nonrecursive Elimination Schemes.
 
 (** State *)
 Record Null_State := { null_state : unit }.
@@ -1050,1171 +1000,6 @@ Qed.
 
 End SimpleContractMorphism.
 
-
-Section TraceMorphism.
-
-(* we introduce the notion of a morphism of chains *)
-
-End TraceMorphism.
-
-
-
-Section ChainMorphism.
-
-(* We introduce the notion of a morphism of chains, which is a morphism on linked lists. *)
-Record ChainMorphism := build_chain_morphism {
-    chainstate_morph : ChainState -> ChainState ; 
-    empty_fixpoint : chainstate_morph empty_state = empty_state ; 
-    chainstep_morph : 
-        forall bstate1 bstate2, 
-        ChainStep bstate1 bstate2 -> 
-        ChainStep (chainstate_morph bstate1) (chainstate_morph bstate2) ;
-}.
-
-(** Composition of chain morphisms *)
-(* an auxiliary lemma *)
-Lemma compose_fixpoint_result (chm1 chm2 : ChainMorphism) : 
-    compose (chainstate_morph chm2) (chainstate_morph chm1) empty_state = 
-    empty_state.
-Proof.
-    unfold compose.
-    rewrite (empty_fixpoint chm1).
-    rewrite (empty_fixpoint chm2).
-    reflexivity.
-Qed.
-
-(* definition of composition *)
-Definition composition_chm (chm2 chm1 : ChainMorphism) : ChainMorphism := {| 
-    chainstate_morph := compose (chainstate_morph chm2) (chainstate_morph chm1) ;
-    empty_fixpoint   := compose_fixpoint_result (chm1) (chm2) ;
-    chainstep_morph  := (fun b1 b2 => 
-        compose 
-            (chainstep_morph chm2 
-                (chainstate_morph chm1 b1) 
-                (chainstate_morph chm1 b2)) 
-            (chainstep_morph chm1 b1 b2)) ;
-|}.
-
-(* composition is associative *)
-Lemma composition_assoc_chm : forall chm1 chm2 chm3, 
-    composition_chm (composition_chm chm3 chm2) chm1 = 
-    composition_chm chm3 (composition_chm chm2 chm1).
-Proof.
-    intros. unfold composition_chm. 
-    f_equal. apply proof_irrelevance.
-Qed.
-
-(* the identity chain morphism *)
-Lemma empty_fixpoint_id : 
-    @id ChainState empty_state = empty_state.
-Proof. auto. Qed.
-
-Definition id_chm : ChainMorphism := {| 
-    chainstate_morph := @id ChainState ; 
-    empty_fixpoint := empty_fixpoint_id ;
-    chainstep_morph := (fun b1 b2 => id_fun (ChainStep b1 b2)) ; |}.
-
-Lemma composition_chm_left : forall chm, composition_chm id_chm chm = chm.
-Proof.
-    intro. unfold composition_chm. 
-    destruct chm. f_equal. apply proof_irrelevance. 
-Qed.
-
-Lemma composition_chm_right : forall chm, composition_chm chm id_chm = chm.
-Proof. 
-    intro. unfold composition_chm. 
-    destruct chm. f_equal. apply proof_irrelevance.
-Qed.
-
-(* chain isomoprhisms, which are bisimulations of blockchains *)
-Definition is_iso_chm (f g : ChainMorphism) : Prop := 
-    composition_chm g f = id_chm /\ 
-    composition_chm f g = id_chm.
-
-(* injections *)
-Definition is_inj_chm (i : ChainMorphism) : Prop :=
-    is_inj (chainstate_morph i).
-
-(* surjections *)
-Definition is_surj_chm (p : ChainMorphism) : Prop :=
-    is_surj (chainstate_morph p).
-
-(* chain monos *)
-Definition is_monic_chm (i : ChainMorphism) : Prop := 
-    forall f f', 
-    composition_chm i f = composition_chm i f' -> f = f'.
-
-(* chain epis *)
-Definition is_epic_chm (p : ChainMorphism) : Prop := 
-    forall f f',
-    composition_chm f p = composition_chm f' p -> f = f'.
-
-(* chain morphisms take reachable states to reachable states *)
-Lemma chm_trace_to_trace : forall bstate1 bstate2 
-    (trace : ChainTrace bstate1 bstate2) (chm : ChainMorphism),
-    ChainTrace (chainstate_morph chm bstate1) (chainstate_morph chm bstate2).
-Proof.
-    intros. destruct chm as [cstate_morph empty_fixpoint cstep_morph]. cbn.
-    induction trace.
-    -   constructor.
-    -   pose proof (cstep_morph mid to l).
-        repeat (econstructor; eauto).
-Qed.
-
-Theorem reachable_to_reachable : forall bstate (chm : ChainMorphism), 
-    reachable bstate -> reachable (chainstate_morph chm bstate).
-Proof.
-    intros.
-    unfold reachable in H. destruct H. unfold reachable.
-    pose proof (chm_trace_to_trace empty_state bstate X chm) as X'.
-    rewrite (empty_fixpoint chm) in X'.
-    constructor.
-    exact X'.
-Qed.
-
-Lemma chm_reachable_through : forall bstate1 bstate2 
-    (trace : reachable_through bstate1 bstate2) (chm : ChainMorphism),
-    reachable_through (chainstate_morph chm bstate1) (chainstate_morph chm bstate2).
-Proof.
-    intros. 
-    destruct trace. unfold reachable_through. destruct H0 as [trace]. split.
-    - exact (reachable_to_reachable bstate1 chm H).
-    - constructor. exact (chm_trace_to_trace bstate1 bstate2 trace chm).
-Qed.
-
-End ChainMorphism.
-
-
-
-Section ReachableChainMorphism.
-
-(* Define the subtype of ChainState which are reachable states *)
-Definition ReachableChainState := {bstate : ChainState | reachable bstate}.
-Definition empty_reachable : ReachableChainState := 
-    exist reachable empty_state reachable_empty_state.
-
-(* We introduce the notion of a morphism of chains, which is a morphism on linked lists. *)
-Record ReachableChainMorphism := build_reachable_chain_morphism {
-    r_chainstate_morph : ReachableChainState -> ReachableChainState ; 
-    r_empty_fixpoint  : r_chainstate_morph empty_reachable = empty_reachable ; 
-    r_chainstep_morph :
-        forall rstate1 rstate2, 
-        ChainStep (proj1_sig rstate1) (proj1_sig rstate2) -> 
-        ChainStep 
-            (proj1_sig (r_chainstate_morph rstate1)) 
-            (proj1_sig (r_chainstate_morph rstate2)) ;
-}.
-
-(** Composition of chain morphisms *)
-(* an auxiliary lemma *)
-Lemma r_compose_fixpoint_result (rchm1 rchm2 : ReachableChainMorphism) : 
-    compose (r_chainstate_morph rchm2) (r_chainstate_morph rchm1) empty_reachable = 
-    empty_reachable.
-Proof.
-    unfold compose.
-    rewrite (r_empty_fixpoint rchm1).
-    rewrite (r_empty_fixpoint rchm2).
-    reflexivity.
-Qed.
-
-(* definition of composition *)
-Definition composition_rchm (rchm2 rchm1 : ReachableChainMorphism) : ReachableChainMorphism := {| 
-    r_chainstate_morph := compose (r_chainstate_morph rchm2) (r_chainstate_morph rchm1) ;
-    r_empty_fixpoint   := r_compose_fixpoint_result (rchm1) (rchm2) ;
-    r_chainstep_morph  := (fun b1 b2 => 
-        compose 
-            (r_chainstep_morph rchm2 
-                (r_chainstate_morph rchm1 b1) 
-                (r_chainstate_morph rchm1 b2)) 
-            (r_chainstep_morph rchm1 b1 b2)) ;
-|}.
-
-(* composition is associative *)
-Lemma composition_assoc_rchm : forall rchm1 rchm2 rchm3, 
-    composition_rchm (composition_rchm rchm3 rchm2) rchm1 = 
-    composition_rchm rchm3 (composition_rchm rchm2 rchm1).
-Proof.
-    intros. unfold composition_rchm.
-    f_equal. apply proof_irrelevance.
-Qed.
-
-(* the identity chain morphism *)
-Lemma r_empty_fixpoint_id : 
-    @id ReachableChainState empty_reachable = empty_reachable.
-Proof. auto. Qed.
-
-Definition id_rchm : ReachableChainMorphism := {| 
-    r_chainstate_morph := @id ReachableChainState ; 
-    r_empty_fixpoint := r_empty_fixpoint_id ;
-    r_chainstep_morph := (fun b1 b2 => id_fun (ChainStep (proj1_sig b1) (proj1_sig b2))) ; |}.
-
-Lemma composition_rchm_left : forall rchm, composition_rchm id_rchm rchm = rchm.
-Proof.
-    intro. unfold composition_rchm. 
-    destruct rchm. f_equal. apply proof_irrelevance.
-Qed.
-
-Lemma composition_rchm_right : forall rchm, composition_rchm rchm id_rchm = rchm.
-Proof. 
-    intro. unfold composition_rchm. 
-    destruct rchm. f_equal. apply proof_irrelevance.
-Qed.
-
-(* chain isomoprhisms, which are bisimulations of blockchains *)
-Definition is_iso_rchm (f g : ReachableChainMorphism) : Prop := 
-    composition_rchm g f = id_rchm /\ 
-    composition_rchm f g = id_rchm.
-
-(* injections *)
-Definition is_inj_rchm (i : ReachableChainMorphism) : Prop :=
-    is_inj (r_chainstate_morph i).
-
-(* surjections *)
-Definition is_surj_rchm (p : ReachableChainMorphism) : Prop :=
-    is_surj (r_chainstate_morph p).
-
-(* chain monos *)
-Definition is_monic_rchm (i : ReachableChainMorphism) : Prop := 
-    forall f f', 
-    composition_rchm i f = composition_rchm i f' -> f = f'.
-
-(* chain epis *)
-Definition is_epic_rchm (p : ReachableChainMorphism) : Prop := 
-    forall f f',
-    composition_rchm f p = composition_rchm f' p -> f = f'.
-
-(* a proof tactic for reachable states *)
-
-Definition rstate_recursion : 
-    forall P : ReachableChainState -> Type,
-    P empty_reachable -> 
-    (forall (rstate : ReachableChainState) (m : P rstate) 
-        (bstate : ChainState) (step : ChainStep (proj1_sig rstate) bstate),
-    P (exist _ bstate (reachable_step (proj1_sig rstate) bstate (proj2_sig rstate) step))) -> 
-    forall rstate : ReachableChainState, P rstate.
-Proof. Admitted.
-
-(* 
-Lemma image_rstate_recursion : forall P img_empty img_rec,
-    rstate_recursion P img_empty img_rec 
-*)
-
-Definition rstate_induction : 
-    forall P : ReachableChainState -> Prop,
-    P empty_reachable -> 
-    (forall (rstate : ReachableChainState) (m : P rstate) 
-        (bstate : ChainState) (step : ChainStep (proj1_sig rstate) bstate),
-    P (exist _ bstate (reachable_step (proj1_sig rstate) bstate (proj2_sig rstate) step)))
-    -> forall rstate : ReachableChainState, P rstate.
-Proof. Admitted.
-
-End ReachableChainMorphism.
-
-Section SimpleMorphismLift.
-Context 
-    { Setup Setup' Msg Msg' State State' Error Error' : Type }
-    `{Serializable Msg}  `{Serializable Setup}  `{Serializable State}  `{Serializable Error}
-    `{Serializable Msg'} `{Serializable Setup'} `{Serializable State'} `{Serializable Error'}
-    {C : Contract Setup Msg State Error} {C' : Contract Setup' Msg' State' Error'}
-    {f : ContractMorphism C C'}.
-
-Axiom inhabitant : forall { T : Type }, inhabited T -> T.
-
-Variable 
-    (* f must be decomposable as follows *)
-    (msg_morph   : Msg   -> Msg')
-    (setup_morph : Setup -> Setup')
-    (state_morph : State -> State')
-    (error_morph : Error -> Error')
-    (* with coherence conditions satisfied *)
-    (init_coherence : forall c ctx s, 
-        (init_result_transform state_morph error_morph) ((init C) c ctx s) = (init C') c ctx (setup_morph s))
-    (recv_coherence : forall c ctx st op_msg, 
-        (recv_result_transform state_morph error_morph) ((receive C) c ctx st op_msg) = 
-        (receive C') c ctx (state_morph st) (option_map msg_morph op_msg))
-    (* f is decomposable *)
-    (f_decomposable : 
-        f = simple_cm msg_morph setup_morph state_morph error_morph init_coherence recv_coherence).
-
-(* TODO *)
-Definition wc_dec_eq : forall w1 w2 : WeakContract, {w1 = w2} + {w1 <> w2}. Admitted.
-Definition wc_eq_bool : WeakContract -> WeakContract -> bool. Admitted.
-Definition wc_eq_bool_op (o1 o2 : option WeakContract) : bool := 
-    match o1, o2 with 
-    | None, None => true 
-    | Some x, Some y => wc_eq_bool x y 
-    | _, _ => false 
-    end.
-Definition wc_eq_bool_spec : 
-    forall (a b : WeakContract), Bool.reflect (a = b) (wc_eq_bool a b). Admitted.
-Declare Scope wc_scope.
-Delimit Scope wc_scope with wc.
-Bind Scope wc_scope with WeakContract.
-Infix "=?" := wc_eq_bool (at level 70) : wc_scope.
-Axiom wc_eq_bool_refl : forall w1 : WeakContract, wc_eq_bool w1 w1 = true.
-
-(* aux functions *)
-Definition C'_deploy : Contract Setup' Msg State' Error' := {| 
-    init := (init C') ; 
-    receive := fun c ctx st o_m => receive C' c ctx st (option_map msg_morph o_m) ;
-|}.
-
-Definition is_c_in_storage (o : option WeakContract) : bool := 
-    match o with 
-    | Some wc => (wc =? contract_to_weak_contract C)%wc
-    | None => false 
-    end.
-
-Definition serialize_map {T T' : Type } `{Serializable T} `{Serializable T'} (f : T -> T') (x : SerializedValue) := 
-    match deserialize x with 
-    | Some ty => (serialize (f ty))
-    | None => x 
-    end.
-
-Definition serialize_result {T E : Type} `{Serializable T} `{Serializable E} 
-    (r : ResultMonad.result T E) : ResultMonad.result SerializedValue SerializedValue := 
-    match r with 
-    | Ok x => Ok (serialize x) 
-    | Err x => Err (serialize x)
-    end.
-
-Definition serialize_result_recv {T T' E : Type} `{Serializable T} `{Serializable E} 
-    (r : ResultMonad.result (T * T') E) : ResultMonad.result (SerializedValue * T') SerializedValue := 
-    match r with 
-    | Ok (x_1, x_2) => Ok (serialize x_1, x_2)
-    | Err x => Err (serialize x)
-    end.
-
-Lemma serialize_init : forall c ctx s rslt,
-    init C' c ctx s = rslt -> 
-    wc_init C' c ctx (serialize s) = serialize_result rslt.
-Admitted.
-
-Lemma serialize_init_preimages : forall c ctx setup state,
-    wc_init (contract_to_weak_contract C) c ctx setup = Ok state -> 
-    (exists (s : Setup), serialize s = setup) /\ 
-    (exists (st : State), serialize st = state).
-Admitted.
-
-Lemma serialize_init_lift : forall c ctx s st, 
-    wc_init (contract_to_weak_contract C) c ctx (serialize s) = Ok (serialize st) -> 
-    init C c ctx s = Ok st.
-Admitted.
-
-Lemma serialize_recv : forall c ctx st m rslt,
-    receive C' c ctx st m = rslt -> 
-    wc_receive C' c ctx (serialize st) (option_map serialize m) = serialize_result_recv rslt.
-Admitted.
-
-Lemma serialize_recv_preimages : forall c ctx prev_state msg new_state resp_acts,
-    wc_receive (contract_to_weak_contract C) c ctx prev_state msg = Ok (new_state, resp_acts) -> 
-    (exists (prev_s : State), serialize prev_s = prev_state) /\ 
-    (exists (new_s  : State), serialize new_s  = new_state)  /\ 
-    (exists (m : option Msg), option_map serialize m = msg).
-Admitted.
-
-Lemma serialize_recv_lift : forall c ctx prev_s m new_s resp_acts, 
-    wc_receive (contract_to_weak_contract C) c ctx (serialize prev_s) (option_map serialize m) 
-        = Ok (serialize new_s, resp_acts) -> 
-    receive C c ctx prev_s m = Ok (new_s, resp_acts).
-Admitted.
-
-Definition action_body_transform (a : ActionBody) (bstate : ChainState) : ActionBody :=
-    match a with 
-        | act_transfer to amt => act_transfer to amt
-        | act_call to amt msg => 
-            if wc_eq_bool_op (env_contracts bstate to) (Some (contract_to_weak_contract C))
-            then act_call to amt (serialize_map msg_morph msg)
-            else act_call to amt msg 
-        | act_deploy amt c setup => 
-            if (c =? contract_to_weak_contract C)%wc
-            then act_deploy amt (contract_to_weak_contract C') (serialize_map setup_morph setup)
-            else act_deploy amt c setup
-    end.
-
-Definition action_transform (a : Action) (bstate : ChainState) : Action := {|
-    act_origin := act_origin a ; 
-    act_from := act_from a ; 
-    act_body := 
-        match act_body a with 
-        | act_transfer to amt => act_transfer to amt
-        | act_call to amt msg =>
-            if wc_eq_bool_op (env_contracts bstate to) (Some (contract_to_weak_contract C))
-            then act_call to amt (serialize_map msg_morph msg)
-            else act_call to amt msg 
-        | act_deploy amt c setup => 
-            if (c =? contract_to_weak_contract C)%wc
-            then act_deploy amt (contract_to_weak_contract C') (serialize_map setup_morph setup)
-            else act_deploy amt c setup
-        end ;
- |}.
-
-Definition wc_transform (wc : WeakContract) : WeakContract := 
-    if (wc =? contract_to_weak_contract C)%wc 
-    then contract_to_weak_contract C' 
-    else wc.
-
-(* the main supporting definitions and lemmas *)
-Definition lift_chainstate_morph (bstate : ChainState) : ChainState := {| 
-    chain_state_env := {| 
-        env_chain := (env_chain bstate) ; 
-        env_account_balances a := (env_account_balances bstate a) ;
-        (* swap out C for C' *)
-        env_contracts a := 
-            if is_c_in_storage (env_contracts bstate a) 
-            then Some (contract_to_weak_contract C') 
-            else  (env_contracts bstate a) ;
-        (* swap out the state of C for its image under state_morph *)
-        env_contract_states a := 
-            if is_c_in_storage (env_contracts bstate a) 
-            then option_map (serialize_map state_morph) (env_contract_states bstate a)
-            else env_contract_states bstate a ;
-    |};
-    chain_state_queue := map (fun x => action_transform x bstate) (chain_state_queue bstate)
-|}.
-
-Lemma lift_empty_fixpoint : lift_chainstate_morph empty_state = empty_state.
-Proof. auto. Qed.
-
-Lemma lift_chainstep_morph : forall bstate1 bstate2, 
-    ChainStep bstate1 bstate2 -> 
-    ChainStep (lift_chainstate_morph bstate1) (lift_chainstate_morph bstate2).
-Proof.
-    intros * step.
-    pose (lift_chainstate_morph bstate1) as bstate1'.
-    pose (lift_chainstate_morph bstate2) as bstate2'.
-    destruct step eqn:HStep.
-        (* step_block *)
-    -   assert (chain_state_queue bstate1' = nil) as e'.
-        1: { simpl. rewrite e. auto. }
-        assert (IsValidNextBlock header bstate1') as i'.
-        1: { simpl. exact i. }
-        assert (Forall act_is_from_account (chain_state_queue bstate2')) as f0'.
-        1: { admit. }
-        assert (Forall act_origin_is_eq_from (chain_state_queue bstate2')) as f1'.
-        1: { simpl. admit. }
-        assert (EnvironmentEquiv bstate2' (add_new_block_to_env header bstate1')) as e0'.
-        1: { simpl. constructor.
-            1: { pose proof (chain_eq bstate2 (add_new_block_to_env header bstate1) e0) as e0''.
-            rewrite e0''. clear e0''. auto. }
-            1: { intro addr.
-            pose proof (account_balances_eq bstate2 (add_new_block_to_env header bstate1) e0 addr) as e0''.
-            cbn. rewrite e0''. auto. }
-            1: { intro addr.
-            pose proof (contracts_eq bstate2 (add_new_block_to_env header bstate1) e0 addr) as e0''.
-            cbn. 
-            rewrite e0''. 
-            auto. }
-            1: { intro addr.
-            pose proof (contract_states_eq bstate2 (add_new_block_to_env header bstate1) e0 addr) as e0''.
-            pose proof (contracts_eq bstate2 (add_new_block_to_env header bstate1) e0 addr) as e0'''.
-            cbn. 
-            rewrite e0''', e0''. 
-            auto. } }
-        exact (step_block bstate1' bstate2' header e' i' f0' f1' e0').
-        (* step_action *)
-    -   pose (action_transform act bstate1) as act'.
-        pose (map (fun x => action_transform x bstate1) acts) as acts'.
-        pose (map (fun x => action_transform x bstate2) new_acts) as new_acts'.
-        assert (chain_state_queue bstate1' = act' :: acts') as e'.
-        1: { unfold act', acts'. cbn. 
-        rewrite e. auto. }
-        assert (ActionEvaluation bstate1' act' bstate2' new_acts') as a'.
-        1: { 
-            destruct a eqn:HEval.
-            (* eval_transfer *)
-            1 : { assert (BinInt.Z.le amount (env_account_balances bstate1' from_addr)) as l'.
-                1: { auto. }
-                assert (act' = {| act_origin := origin; act_from := from_addr; act_body := act_transfer to_addr amount |}) as e2'.
-                1: { unfold act', action_transform. rewrite e2. cbn. auto. }
-                assert (EnvironmentEquiv bstate2' (transfer_balance from_addr to_addr amount bstate1')) as e3'. 
-                1: { simpl. constructor.
-                    -   apply e3. 
-                    -   intro addr. apply e3. 
-                    -   intro addr.
-                        pose proof (contracts_eq bstate2 (transfer_balance from_addr to_addr amount bstate1) e3 addr) as e''. 
-                        cbn.
-                        rewrite e''. 
-                        auto. 
-                    -   intro addr.
-                        pose proof (contract_states_eq bstate2 (transfer_balance from_addr to_addr amount bstate1) e3 addr) as e''.
-                        pose proof (contracts_eq bstate2 (transfer_balance from_addr to_addr amount bstate1) e3 addr) as e'''.
-                        cbn. 
-                        rewrite e''', e''. 
-                        auto. }
-                assert (new_acts' = nil) as e4'.
-                1: { unfold new_acts'. rewrite e4. auto. }
-                exact (eval_transfer origin from_addr to_addr amount g l' e1 e2' e3' e4'). }
-            (* eval_deploy *)
-            1 : { pose (wc_transform wc) as wc'.
-                pose (if (wc =? contract_to_weak_contract C)%wc 
-                    then serialize_map setup_morph setup
-                    else setup) as setup'.
-                pose (if (wc =? contract_to_weak_contract C)%wc 
-                    then serialize_map state_morph state
-                    else state) as state'.
-                assert (BinInt.Z.le amount (env_account_balances bstate1' from_addr)) as l'.
-                1: { auto. }
-                assert (env_contracts bstate1' to_addr = None) as e2'.
-                1: { cbn. 
-                    destruct (is_c_in_storage (env_contracts bstate1 to_addr)) eqn:H_is_c; auto.
-                    unfold is_c_in_storage in H_is_c.
-                    rewrite e2 in H_is_c.
-                    inversion H_is_c. }
-                assert (act' = {| act_origin := origin; act_from := from_addr; act_body := act_deploy amount wc' setup' |}) as e3'.
-                1: { unfold act', action_transform, wc', wc_transform, setup'.
-                    rewrite e3. cbn. f_equal.
-                    destruct ((wc =? C)%wc); auto. }
-                (* here we use the coherence conditions of f *)
-                assert (wc_init wc' (transfer_balance from_addr to_addr amount bstate1')
-                    {|
-                    ctx_origin := origin;
-                    ctx_from := from_addr;
-                    ctx_contract_address := to_addr;
-                    ctx_contract_balance := amount;
-                    ctx_amount := amount
-                    |} setup' = Ok state') as e4'.
-                1: { simpl. simpl in e4.
-                    unfold wc', setup', state', wc_transform.
-                    set {| ctx_origin := origin; ctx_from := from_addr;
-                           ctx_contract_address := to_addr; ctx_contract_balance := amount;
-                           ctx_amount := amount |} as ctx.
-                    destruct (wc =? C)%wc eqn:H_wc; try apply e4.
-                    (* derive equality from boolean equality *)
-                    pose proof (wc_eq_bool_spec wc C).
-                    apply reflect_iff in H7. 
-                    rewrite <- H7 in H_wc. clear H7. 
-                    (* get the preimage of setup and state *)
-                    pose proof (serialize_init_preimages bstate1 ctx setup state) as lemma_init_preimages.
-                    rewrite <- H_wc in lemma_init_preimages.
-                    set e4 as init_preimages.
-                    apply lemma_init_preimages in init_preimages. clear lemma_init_preimages.
-                    destruct init_preimages as [exists_s exists_st].
-                    destruct exists_s as [s ser_s].
-                    destruct exists_st as [st ser_st].
-                    pose proof (init_coherence bstate1 ctx s) as init_coh.
-                    pose proof (serialize_init bstate1 ctx (setup_morph s) (init_result_transform state_morph error_morph (init C bstate1 ctx s))) as serialize_init_coh.
-                    symmetry in init_coh.
-                    apply serialize_init_coh in init_coh. clear serialize_init_coh.
-                    assert ((serialize_map setup_morph setup) = (serialize (setup_morph s))) as ser_comm.
-                    1: { unfold serialize_map. rewrite <- ser_s. rewrite deserialize_serialize. auto. }
-                    (* apply init coherence *)
-                    rewrite ser_comm.
-                    rewrite init_coh.
-                    unfold serialize_result, serialize_map, init_result_transform.
-                    (* rewrite e4 *)
-                    pose proof (serialize_init_lift bstate1 ctx s st) as c_init_lift.
-                    rewrite ser_s, ser_st in c_init_lift.
-                    assert (init C bstate1 ctx s = Ok st) as e4_lift.
-                    1: { apply c_init_lift. 
-                        rewrite <- H_wc. 
-                        exact e4. }
-                    rewrite e4_lift.
-                    rewrite <- ser_st.
-                    rewrite deserialize_serialize.
-                    auto. }
-                assert (EnvironmentEquiv bstate2'
-                    (set_contract_state to_addr state'
-                    (add_contract to_addr wc' (transfer_balance from_addr to_addr amount bstate1')))) as e5'.
-                1: { simpl. constructor.
-                    -   apply e5.
-                    -   intro addr. apply e5.
-                    -   intro addr.
-                        pose proof (contracts_eq bstate2 (set_contract_state to_addr state
-                        (add_contract to_addr wc (transfer_balance from_addr to_addr amount bstate1))) e5 addr) as e''.
-                        cbn.
-                        rewrite e''. 
-                        simpl.
-                        destruct (addr =? to_addr)%address; auto.
-                        unfold wc', wc_transform, is_c_in_storage.
-                        destruct (wc =? C)%wc; auto.
-                    -   intro addr. simpl.
-                        unfold is_c_in_storage.
-                        pose proof (contract_states_eq bstate2 (set_contract_state to_addr state
-                        (add_contract to_addr wc (transfer_balance from_addr to_addr amount bstate1))) e5 addr) as e''.
-                        pose proof (contracts_eq bstate2 (set_contract_state to_addr state
-                        (add_contract to_addr wc (transfer_balance from_addr to_addr amount bstate1))) e5 addr) as e'''.
-                        rewrite e'', e'''. simpl.
-                        unfold state'.
-                        destruct (addr =? to_addr)%address; auto.
-                        simpl.
-                        destruct (wc =? C)%wc; auto. }
-                assert (new_acts' = nil) as e6'.
-                1: { unfold new_acts'. rewrite e6. unfold action_transform. auto. }
-                exact (eval_deploy origin from_addr to_addr amount wc' setup' state' g l' e1 e2' e3' e4' e5' e6'). }
-            (* eval_call *)
-            1 : { pose (wc_transform wc) as wc'.
-                pose (if (wc_eq_bool_op (env_contracts bstate1 to_addr) (Some (contract_to_weak_contract C)))
-                    then option_map (serialize_map msg_morph) msg
-                    else msg) as msg'.
-                pose (if (wc =? contract_to_weak_contract C)%wc 
-                    then serialize_map state_morph prev_state
-                    else prev_state) as prev_state'.
-                pose (if (wc =? contract_to_weak_contract C)%wc 
-                    then serialize_map state_morph new_state
-                    else new_state) as new_state'.
-                pose (map (fun x => action_body_transform x bstate1) resp_acts) as resp_acts'.
-                assert (BinInt.Z.le amount (env_account_balances bstate1' from_addr)) as l'.
-                1: { auto. }
-                assert (env_contracts bstate1' to_addr = Some wc') as e1'.
-                1: { cbn. unfold wc', wc_transform.
-                    destruct (is_c_in_storage (env_contracts bstate1 to_addr)) eqn:H_is_c.
-                    -   unfold is_c_in_storage in H_is_c.
-                        rewrite e1 in H_is_c.
-                        rewrite H_is_c; auto.
-                    -   unfold is_c_in_storage in H_is_c.
-                        rewrite e1 in H_is_c.
-                        rewrite H_is_c. 
-                        exact e1. }
-                assert (env_contract_states bstate1' to_addr = Some prev_state') as e2'.
-                1: { cbn. unfold prev_state', is_c_in_storage.
-                    replace (env_contracts bstate1 to_addr) with (Some wc).
-                    cbn.
-                    destruct (wc =? C)%wc; auto.
-                    rewrite e2; auto. }
-                assert (act' = {|
-                    act_origin := origin;
-                    act_from := from_addr;
-                    act_body := match msg' with
-                                | Some msg' => act_call to_addr amount msg'
-                                | None => act_transfer to_addr amount
-                                end |}) as e3'.
-                1: { unfold act'. unfold action_transform.
-                    rewrite e3. cbn. 
-                    f_equal.
-                    unfold msg'. rewrite e1.
-                    destruct msg; cbn; destruct (wc =? C)%wc eqn:H_wc_eq; auto.
-                    -   pose proof (wc_eq_bool_spec wc C).
-                        apply reflect_iff in H7.
-                        rewrite <- H7 in H_wc_eq.
-                        rewrite <- H_wc_eq. rewrite e1. cbn.
-                        rewrite wc_eq_bool_refl. auto.
-                    -   unfold wc_eq_bool_op. 
-                        rewrite e1. rewrite H_wc_eq. 
-                        auto. }
-                (* here we use the coherence conditions of f *)
-                assert (wc_receive wc' (transfer_balance from_addr to_addr amount bstate1')
-                {|
-                  ctx_origin := origin;
-                  ctx_from := from_addr;
-                  ctx_contract_address := to_addr;
-                  ctx_contract_balance := env_account_balances bstate2' to_addr;
-                  ctx_amount := amount
-                |} prev_state' msg' = Ok (new_state', resp_acts')) as e4'.
-                1: { simpl. simpl in e4.
-                    set {| ctx_origin := origin;
-                        ctx_from := from_addr;
-                        ctx_contract_address := to_addr;
-                        ctx_contract_balance := env_account_balances bstate2 to_addr;
-                        ctx_amount := amount |} as ctx.
-                    unfold wc', prev_state', msg', new_state'.
-                    destruct (wc =? C)%wc eqn:H_wc.
-                    (* first the case that wc <> C *)
-                    2: { (* derive equality from boolean equality *)
-                    pose proof (wc_eq_bool_spec wc C).
-                    apply reflect_iff in H7.
-                    assert ((wc =? C)%wc <> true) as H_wc'.
-                    1: { unfold not. intro. rewrite H_wc in H8. discriminate. }
-                    rewrite <- H7 in H_wc'. clear H7.
-                    unfold wc_transform. rewrite H_wc.
-                    unfold wc_eq_bool_op. rewrite e1. rewrite H_wc.
-                    unfold ctx. rewrite e4.
-                    repeat f_equal.
-                    admit. }
-                    (* now the case that wc = C *)
-                    (* derive equality from boolean equality *)
-                    pose proof (wc_eq_bool_spec wc C).
-                    set H_wc as H_wc'.
-                    apply reflect_iff in H7.
-                    rewrite <- H7 in H_wc'. clear H7.
-                    rewrite H_wc'. unfold wc_transform. rewrite wc_eq_bool_refl.
-                    unfold wc_eq_bool_op. rewrite e1. rewrite H_wc.
-                    (* get the preimage of prev_state msg new_state *)
-                    pose proof (serialize_recv_preimages bstate1 ctx prev_state msg new_state resp_acts) as lemma_recv_preimages.
-                    unfold ctx in lemma_recv_preimages.
-                    rewrite <- H_wc' in lemma_recv_preimages.
-                    set e4 as recv_preimages.
-                    apply lemma_recv_preimages in recv_preimages. clear lemma_recv_preimages.
-                    destruct recv_preimages as [exists_ps recv_preimages].
-                    destruct recv_preimages as [exists_ns exists_m].
-                    destruct exists_ps as [prev_s ser_prev_s].
-                    destruct exists_ns as [new_s  ser_new_s].
-                    destruct exists_m as [m ser_m].
-                    pose proof (recv_coherence bstate1 ctx prev_s m) as recv_coh.
-                    pose proof (serialize_recv bstate1 ctx (state_morph prev_s) (option_map msg_morph m) (recv_result_transform state_morph error_morph (receive C bstate1 ctx prev_s m))) as serialize_recv_coh.
-                    symmetry in recv_coh.
-                    apply serialize_recv_coh in recv_coh. clear serialize_recv_coh.
-                    assert ((serialize_map state_morph prev_state) = (serialize (state_morph prev_s))) as ser_comm1.
-                    1: { unfold serialize_map. rewrite <- ser_prev_s. rewrite deserialize_serialize. auto. }
-                    assert ((option_map (serialize_map msg_morph) msg) = (option_map serialize (option_map msg_morph m))) as ser_comm2.
-                    1: { rewrite <- ser_m. unfold option_map, serialize_map.
-                        destruct m; auto. 
-                        rewrite deserialize_serialize. 
-                        auto. }
-                    (* apply recv coherence *)
-                    rewrite ser_comm1, ser_comm2.
-                    rewrite recv_coh.
-                    unfold serialize_result_recv, serialize_map, recv_result_transform.
-                    (* rewrite e4 *)
-                    pose proof (serialize_recv_lift bstate1 ctx prev_s m new_s resp_acts) as c_recv_lift.
-                    rewrite ser_prev_s, ser_new_s, ser_m in c_recv_lift.
-                    assert (receive C bstate1 ctx prev_s m = Ok (new_s, resp_acts)) as e4_lift.
-                    1: { apply c_recv_lift.
-                        rewrite <- H_wc'.
-                        exact e4. }
-                    rewrite e4_lift.
-                    rewrite <- ser_new_s. rewrite deserialize_serialize.
-                    repeat f_equal.
-                    admit. }
-                assert (new_acts' = map (build_act origin to_addr) resp_acts') as e5'.
-                1: { unfold new_acts', resp_acts'.
-                    rewrite e5.
-                    assert (forall l, map (fun x => action_transform x bstate1) (map (build_act origin to_addr) l) =
-                    map (build_act origin to_addr) (map (fun x => action_body_transform x bstate1) l)) as H_act.
-                    1: { intro. induction l0; auto. 
-                        repeat rewrite map_cons.
-                        f_equal. auto. }
-                    rewrite <- (H_act resp_acts).
-                    assert (forall bstate1 bstate2 (step : ChainStep bstate1 bstate2), 
-                        map (fun x : Action => action_transform x bstate2) 
-                            (map (build_act origin to_addr) resp_acts) =
-                        map (fun x : Action => action_transform x bstate1) 
-                            (map (build_act origin to_addr) resp_acts)) as acts_equiv.
-                    1: { admit. }
-                    rewrite (acts_equiv bstate1 bstate2 step).
-                    auto. }
-                assert (EnvironmentEquiv bstate2' (set_contract_state to_addr new_state' (transfer_balance from_addr to_addr amount bstate1'))) as e6'.
-                1: { simpl. constructor.
-                    -   apply e6.
-                    -   intro addr. apply e6.
-                    -   intro addr. 
-                        pose proof ((contracts_eq bstate2 (set_contract_state to_addr new_state (transfer_balance from_addr to_addr amount bstate1))) e6 addr) as e''.
-                        cbn.
-                        rewrite e''. 
-                        auto.
-                    -   intro addr. simpl.
-                        unfold is_c_in_storage, new_state'.
-                        pose proof (contract_states_eq bstate2 (set_contract_state to_addr new_state (transfer_balance from_addr to_addr amount bstate1)) e6 addr) as e''.
-                        pose proof (contracts_eq bstate2 (set_contract_state to_addr new_state (transfer_balance from_addr to_addr amount bstate1)) e6 addr) as e'''.
-                        rewrite e'', e'''. simpl.
-                        destruct (addr =? to_addr)%address eqn:H_addr; auto.
-                        pose proof (address_eqb_spec addr to_addr) as H_addr_eq. 
-                        apply reflect_iff in H_addr_eq. 
-                        rewrite <- H_addr_eq in H_addr.
-                        rewrite H_addr. rewrite e1.
-                        destruct (wc =? C)%wc; cbn; auto. }
-                exact (eval_call origin from_addr to_addr amount wc' msg' prev_state' new_state' resp_acts' g l' e1' e2' e3' e4' e5' e6'). } }
-        assert (chain_state_queue bstate2' = new_acts' ++ acts') as e0'. 
-        1: { unfold new_acts', acts'. cbn.
-            rewrite e0.
-            assert (forall bstate1 bstate2 (step : ChainStep bstate1 bstate2) acts, 
-            map (fun x : Action => action_transform x bstate1) acts = 
-            map (fun x : Action => action_transform x bstate2) acts) as acts_equiv.
-            1: { admit. }
-            rewrite (acts_equiv bstate1 bstate2 step acts).
-            apply map_app. }
-        exact (step_action bstate1' bstate2' act' acts' new_acts' e' a' e0').
-        (* step_action_indvalid *)
-    -   pose (action_transform act bstate1) as act'.
-        pose (map (fun x => action_transform x bstate1) acts) as acts'.
-        assert (EnvironmentEquiv bstate2' bstate1') as e'.
-        1: { simpl. constructor. 
-            1: { pose proof (chain_eq bstate2 bstate1 e) as e''.
-            rewrite e''. clear e''. auto. }
-            1: { intro addr.
-            pose proof (account_balances_eq bstate2 bstate1 e addr) as e''.
-            cbn. rewrite e''. auto. }
-            1: { intro addr.
-            pose proof (contracts_eq bstate2 bstate1 e addr) as e''.
-            cbn. 
-            rewrite e''. 
-            auto. }
-            1: { intro addr.
-            pose proof (contract_states_eq bstate2 bstate1 e addr) as e''.
-            pose proof (contracts_eq bstate2 bstate1 e addr) as e'''.
-            cbn. 
-            rewrite e''', e''. 
-            auto. } }
-        assert (chain_state_queue bstate1' = act' :: acts') as e0'. 
-        1: { unfold act', acts'. cbn. rewrite e0. auto. }
-        assert (chain_state_queue bstate2' = acts') as e1'. 
-        1: { unfold acts'. cbn. rewrite e1. auto.
-            assert (forall bstate1 bstate2 (step : ChainStep bstate1 bstate2) acts,
-                map (fun x : Action => action_transform x bstate1) acts = 
-                map (fun x : Action => action_transform x bstate2) acts) as acts_equiv. 
-            1: { admit. }
-            rewrite (acts_equiv bstate1 bstate2 step acts).
-            auto. }
-        assert (act_is_from_account act') as a'. 
-        1: { unfold act_is_from_account, act'. simpl. apply a. }
-        assert (forall (bstate : Environment) (new_acts : list Action), 
-            ActionEvaluation bstate1' act' bstate new_acts -> False) as f0'. 
-        1: { intros * false_eval.
-            destruct false_eval eqn:HEval;
-            (* TODO construct a preimage bstate *)
-            apply (f0 bstate new_acts).
-            (* Construct preimages for each type of ActionEvaluation *)
-            (* eval_transfer *)
-            1 : { assert (BinInt.Z.le amount (env_account_balances bstate1 from_addr)) as l'.
-                1: { unfold bstate1' in l. cbn in l. exact l. }
-                assert (act = {| act_origin := origin; act_from := from_addr; act_body := act_transfer to_addr amount |}) as e3'.
-                1 : { destruct act.
-                    unfold act' in e3.
-                    inversion e3.
-                    f_equal.
-                    destruct act_body eqn:H_body; auto.
-                    -   inversion e3. 
-                        destruct (wc_eq_bool_op (env_contracts bstate1 to) (Some (C : WeakContract)));
-                        inversion H13.
-                    -   inversion e3.
-                        destruct (c =? C)%wc;
-                        inversion H13. }
-                assert (EnvironmentEquiv bstate (transfer_balance from_addr to_addr amount bstate1)) as e4'.
-                1: { simpl. constructor; destruct e4.
-                    -   rewrite chain_eq.
-                        auto.
-                    -   intro addr.
-                        pose proof (account_balances_eq addr).
-                        rewrite H7. 
-                        auto.
-                    -   intro addr.
-                        pose proof (contracts_eq addr).
-                        rewrite H7.
-                        cbn.
-                        destruct (is_c_in_storage (env_contracts bstate1 addr)); auto.
-                        (* TODO not sure how to handle the EnvironmentEquiv bit ...
-                            probably need to generalize or something. or find a preimage of bstate *)
-                        admit.
-                    -   intro addr.
-                        pose proof (contract_states_eq addr).
-                        rewrite H7.
-                        cbn.
-                        destruct (is_c_in_storage (env_contracts bstate1 addr)); auto.
-                        admit. }
-                (* the corresponding action in ActionEvaluation bstate1 act bstate new_acts *)
-                exact (eval_transfer origin from_addr to_addr amount g l' e2 e3' e4' e5). }
-            (* eval_deploy *)
-            1 : { pose (wc_transform wc) as wc'.
-                assert (SerializedValue) as setup'.
-                1: { admit. }
-                assert (SerializedValue) as state'.
-                1: { admit. }
-                assert (BinInt.Z.le amount (env_account_balances bstate1 from_addr)) as l'.
-                1: { admit. }
-                assert (env_contracts bstate1 to_addr = None) as e3'.
-                1: { admit. }
-                assert (act = {| act_origin := origin; act_from := from_addr; act_body := act_deploy amount wc' setup' |}) as e4'.
-                1: { admit. }
-                pose {| ctx_origin := origin;
-                        ctx_from := from_addr;
-                        ctx_contract_address := to_addr;
-                        ctx_contract_balance := amount;
-                        ctx_amount := amount |} as ctx.
-                assert (wc_init wc' (transfer_balance from_addr to_addr amount bstate1) ctx setup' 
-                    = Ok state') as e5'.
-                1: { admit. }
-                assert (EnvironmentEquiv bstate
-                (set_contract_state to_addr state' (add_contract to_addr wc' (transfer_balance from_addr to_addr amount bstate1)))) as e6'.
-                1: { admit. }
-                exact (eval_deploy origin from_addr to_addr amount wc' setup' state' g l' e2 e3' e4' e5' e6' e7). }
-            (* eval_call *)
-            1 : { pose (wc_transform wc) as wc'.
-                assert (option SerializedValue) as msg'.
-                1: { admit. }
-                assert (SerializedValue) as prev_state'.
-                1: { admit. }
-                assert (SerializedValue) as new_state'.
-                1: { admit. }
-                assert (BinInt.Z.le amount (env_account_balances bstate1 from_addr)) as l'.
-                1: { admit. }
-                assert (env_contracts bstate1 to_addr = Some wc') as e2'.
-                1: { admit. }
-                assert (env_contract_states bstate1 to_addr = Some prev_state') as e3'.
-                1: { admit. }
-                assert (act =
-                {|
-                  act_origin := origin;
-                  act_from := from_addr;
-                  act_body := match msg' with
-                              | Some msg => act_call to_addr amount msg
-                              | None => act_transfer to_addr amount
-                              end
-                |}) as e4'.
-                1: { admit. }
-                pose {|
-                    ctx_origin := origin;
-                    ctx_from := from_addr;
-                    ctx_contract_address := to_addr;
-                    ctx_contract_balance := env_account_balances bstate to_addr;
-                    ctx_amount := amount
-                  |} as ctx.
-                assert (wc_receive wc' (transfer_balance from_addr to_addr amount bstate1)
-                    ctx prev_state' msg' = Ok (new_state', resp_acts)) as e5'.
-                1: { admit. }
-                assert (EnvironmentEquiv bstate (set_contract_state to_addr new_state' (transfer_balance from_addr to_addr amount bstate1))) as e7'.
-                1: { admit. }
-                exact (eval_call origin from_addr to_addr amount wc' msg' prev_state' new_state' resp_acts g l' e2' e3' e4' e5' e6 e7'). } }
-        exact (step_action_invalid bstate1' bstate2' act' acts' e' e0' e1' a' f0').
-        (* step_permute *)
-    -   assert (EnvironmentEquiv bstate2' bstate1') as e'.
-        1: { simpl. constructor.
-            1: { pose proof (chain_eq bstate2 bstate1 e) as e''.
-            rewrite e''. clear e''. auto. }
-            1: { intro addr.
-            pose proof (account_balances_eq bstate2 bstate1 e addr) as e''.
-            cbn. rewrite e''. auto. }
-            1: { intro addr.
-            pose proof (contracts_eq bstate2 bstate1 e addr) as e''.
-            cbn. 
-            rewrite e''. 
-            auto. }
-            1: { intro addr.
-            pose proof (contract_states_eq bstate2 bstate1 e addr) as e''.
-            pose proof (contracts_eq bstate2 bstate1 e addr) as e'''.
-            cbn. 
-            rewrite e''', e''. 
-            auto. } }
-        assert (Permutation (chain_state_queue bstate1') (chain_state_queue bstate2')) as p'.
-        1: { simpl. admit. }
-        exact (step_permute bstate1' bstate2' e' p').
-Admitted.
-
-(* the main function *)
-Definition simple_cm_lift_to_chm : ChainMorphism := 
-    build_chain_morphism
-        lift_chainstate_morph
-        lift_empty_fixpoint
-        lift_chainstep_morph.
-
-(* the swap corrolary *)
-Corollary c_c'_swap : 
-    forall (bstate : ChainState) (caddr : Address),
-    env_contracts bstate caddr = Some (C : WeakContract) -> 
-    env_contracts (chainstate_morph simple_cm_lift_to_chm bstate) caddr = Some (C' : WeakContract).
-Proof.
-    intros. cbn.
-    unfold is_c_in_storage. rewrite H7.
-    rewrite (wc_eq_bool_refl C).
-    reflexivity.
-Qed.
-
-End SimpleMorphismLift.
-
-(** We now examine how lifted morphisms behave with regard to morphism composition *)
-Section ContractMorphismLiftCompose.
-Context 
-    { Setup Setup' Msg Msg' State State' Error Error' : Type }
-    `{Serializable Msg}  `{Serializable Setup}  `{Serializable State}  `{Serializable Error}
-    `{Serializable Msg'} `{Serializable Setup'} `{Serializable State'} `{Serializable Error'}
-    {C : Contract Setup Msg State Error} {C' : Contract Setup' Msg' State' Error'}
-    {f : ContractMorphism C C'}.
-
-(* TODO resolve simplicity parameters somehow. Make this easy for future use! *)
-
-(* id_cm lifts to id_chm *)
-Lemma id_cm_to_id_chm 
-    { Setup Msg State Error : Type }
-    `{Serializable Msg} `{Serializable Setup} `{Serializable State} `{Serializable Error}
-    { C : Contract Setup Msg State Error } : 
-    simple_cm_lift_to_chm (id_cm C) = id_chm.
-Proof. Admitted.
-
-(* compositions lift to compositions *)
-Lemma cm_lift_compose 
-    { Setup Setup' Setup'' Msg Msg' Msg'' State State' State'' Error Error' Error'' : Type }
-    `{Serializable Msg}    `{Serializable Setup}    `{Serializable State}    `{Serializable Error}
-    `{Serializable Msg'}   `{Serializable Setup'}   `{Serializable State'}   `{Serializable Error'}
-    `{Serializable Msg''}  `{Serializable Setup''}  `{Serializable State''}  `{Serializable Error''}
-    { C : Contract Setup Msg State Error } 
-    { C' : Contract Setup' Msg' State' Error' }
-    { C'' : Contract Setup'' Msg'' State'' Error'' } : 
-    forall (f : ContractMorphism C C') (g : ContractMorphism C' C''),
-    composition_chm (simple_cm_lift_to_chm g) (simple_cm_lift_to_chm f) = 
-    simple_cm_lift_to_chm (composition_cm g f).
-Proof. Admitted.
-
-(* isomorphisms lift to isomorphisms *)
-Lemma iso_cm_to_iso_chm 
-    { Setup Setup' Msg Msg' State State' Error Error' : Type }
-    `{Serializable Msg} `{Serializable Setup} `{Serializable State} `{Serializable Error}
-    `{Serializable Msg'} `{Serializable Setup'} `{Serializable State'} `{Serializable Error'}
-    { C : Contract Setup Msg State Error } 
-    { C' : Contract Setup' Msg' State' Error' } : 
-    forall (f : ContractMorphism C C') (g : ContractMorphism C' C), 
-    is_iso_cm f g -> 
-    is_iso_chm (simple_cm_lift_to_chm f) (simple_cm_lift_to_chm g).
-Proof.
-    intros * is_iso.
-    unfold is_iso_chm. unfold is_iso_cm in is_iso. 
-    destruct is_iso as [iso_to iso_from].
-    split.
-    -   rewrite (cm_lift_compose f g). rewrite iso_to. 
-        rewrite id_cm_to_id_chm. reflexivity.
-    -   rewrite (cm_lift_compose g f). rewrite iso_from.   
-        rewrite id_cm_to_id_chm. reflexivity.
-Qed.
-
-(* TODO 
-Lemma inj_lifts_to_inj
-Lemma surj_lifts_to_surj
-*)
-
-End ContractMorphismLiftCompose.
-
-
-Section Equivalences.
-
-(* equivalence of contracts *)
-Definition are_equiv 
-    { Setup Setup' Msg Msg' State State' Error Error' : Type }
-    `{Serializable Msg} `{Serializable Setup} `{Serializable State} `{Serializable Error}
-    `{Serializable Msg'} `{Serializable Setup'} `{Serializable State'} `{Serializable Error'}
-    (C  : Contract Setup  State  Msg  Error)
-    (C' : Contract Setup' State' Msg' Error') : Prop := 
-    exists (f : ContractMorphism C C') (g : ContractMorphism C' C),
-    is_iso_cm f g.
-
-(* weak equivalence of contracts *)
-Definition are_weakly_equiv 
-    { Setup Setup' Msg Msg' State State' Error Error' : Type }
-    `{Serializable Msg} `{Serializable Setup} `{Serializable State} `{Serializable Error}
-    `{Serializable Msg'} `{Serializable Setup'} `{Serializable State'} `{Serializable Error'}
-    (C  : Contract Setup  State  Msg  Error)
-    (C' : Contract Setup' State' Msg' Error') : Prop := 
-    exists (f g : ChainMorphism), 
-    is_iso_chm f g /\
-    forall (bstate : ChainState) caddr, 
-    (env_contracts bstate caddr = Some (C : WeakContract)  
-        -> env_contracts (chainstate_morph f bstate) caddr = Some (C' : WeakContract)) /\
-    (env_contracts bstate caddr = Some (C' : WeakContract) 
-        -> env_contracts (chainstate_morph g bstate) caddr = Some (C : WeakContract)).
-
-End Equivalences.
-
-(** Contract Morphisms lift to Reachable Chain Morphisms *)
-(*
-Section ReachableMorphismLift.
-Context 
-    { Setup Setup' Msg Msg' State State' Error Error' : Type }
-    `{Serializable Msg}  `{Serializable Setup}  `{Serializable State}  `{Serializable Error}
-    `{Serializable Msg'} `{Serializable Setup'} `{Serializable State'} `{Serializable Error'}
-    {C : Contract Setup Msg State Error} {C' : Contract Setup' Msg' State' Error'}.
-
-(* preparatory lemmata and functions *)
-
-(* construct a ReachableChainMorphism in three pieces *)
-Definition cm_to_reachable_chainstate_morph (f : ContractMorphism C C') : 
-    ReachableChainState -> ReachableChainState.
-Admitted. 
-    apply rstate_recursion.
-    -   exact empty_reachable.
-    -   intros rstate1 rstate1' bstate2 cstep.
-        destruct rstate1 as [bstate1 trace1].
-        destruct rstate1' as [bstate1' trace1']. 
-        simpl in cstep.
-        destruct cstep eqn:HS.
-        +   pose bstate1' as bstate2'.
-            assert (ChainStep bstate1' bstate2') as step'.
-            2: {
-                pose proof (reachable_step bstate1' bstate2' trace1' step') as trace2'.
-                exact (exist _ bstate2' trace2').
-            }
-            apply (step_block bstate1' bstate2' header).
-            *   
-            *      
-            *   
-            *   
-            *   
-        +   
-        +   
-        +   
-
-
-Definition cm_to_reachable_chainstate_morph (f : ContractMorphism C C')
-    (rstate : ReachableChainState) : ReachableChainState.
-Proof.
-    destruct rstate as [rstate1 trace].
-    unfold reachable in trace. apply inhabitant in trace.
-    induction trace eqn:HR.
-    -   exact empty_reachable.
-    -   pose (IHc c (reflexivity c)) as rstate1'.
-        induction l eqn:HL.
-        +   admit.
-        +   admit.
-        +   admit.
-        +   admit.
-Admitted.
-
-Lemma lift_empty_fixpoint (f : ContractMorphism C C') :
-    cm_to_reachable_chainstate_morph f empty_reachable = empty_reachable.
-Admitted.
-
-Lemma lift_chainstep_morph (f : ContractMorphism C C') : 
-    forall rstate1 rstate2, 
-    ChainStep (proj1_sig rstate1) (proj1_sig rstate2) -> 
-    ChainStep 
-        (proj1_sig (cm_to_reachable_chainstate_morph f rstate1)) 
-        (proj1_sig (cm_to_reachable_chainstate_morph f rstate2)).
-Admitted.
-
-(* the lifting result *)
-Definition cm_lift_to_rchm (f : ContractMorphism C C') : ReachableChainMorphism := 
-    build_reachable_chain_morphism
-        (cm_to_reachable_chainstate_morph f)
-        (lift_empty_fixpoint f)
-        (lift_chainstep_morph f).
-
-(* the swap result *)
-Theorem c_c'_swap : 
-    forall (rstate : ReachableChainState) (caddr : Address) (f : ContractMorphism C C'),
-    let rstate' := r_chainstate_morph (cm_lift_to_rchm f) rstate in 
-    env_contracts (proj1_sig rstate)  caddr = Some (C  : WeakContract) -> 
-    env_contracts (proj1_sig rstate') caddr = Some (C' : WeakContract).
-Proof.
-    intros.
-Admitted.
-
-End ReachableMorphismLift.
-*)
-
-(* 
-(** Simple Contract Morphisms lift to Chain Morphisms *)
-Section ContractMorphismLift.
-Context 
-    { Setup Setup' Msg Msg' State State' Error Error' : Type }
-    `{Serializable Msg}  `{Serializable Setup}  `{Serializable State}  `{Serializable Error}
-    `{Serializable Msg'} `{Serializable Setup'} `{Serializable State'} `{Serializable Error'}
-    {C : Contract Setup Msg State Error} {C' : Contract Setup' Msg' State' Error'}.
-
-the lifting function 
-Definition lift_chainstate_morph (f : ContractMorphism C C') : ChainState -> ChainState := todo "".
-    (*  *)
-    
-Lemma lift_empty_fixpoint (f : ContractMorphism C C') : 
-    lift_chainstate_morph f empty_state = empty_state. Admitted.
-
-Definition lift_chainstep_morph (f : ContractMorphism C C') : 
-    forall bstate1 bstate2, 
-    ChainStep bstate1 bstate2 -> 
-    ChainStep 
-        (lift_chainstate_morph f bstate1) (lift_chainstate_morph f bstate2) := todo "".
-
-(* the main function *)
-Definition simple_cm_lift_to_chm (f : ContractMorphism C C') : ChainMorphism :=
-    build_chain_morphism
-        (lift_chainstate_morph f)
-        (lift_empty_fixpoint f)
-        (lift_chainstep_morph f).
-
-Lemma c_c'_swap : 
-    forall (bstate : ChainState) (caddr : Address) (f : ContractMorphism C C'),
-    env_contracts bstate caddr = Some (C : WeakContract) -> 
-    env_contracts (chainstate_morph (simple_cm_lift_to_chm f) bstate) caddr = Some (C' : WeakContract).
-Proof.
-    intros.
-Admitted.
-End ContractMorphismLift.
-*)
 
 
 End ContractMorphisms.
